#+AUTHOR: Aryan Pandey
#+TITLE: Nonlinear Programming
#+HTML_HEAD: <link rel="stylesheet" type="text/css" href="../../worg.css"/>
* NLPP with one equality constraint (two or three variables) using the method of Lagrangeâ€™s multipliers
\begin{equation}
h = constraint
\end{equation}
\begin{equation}
L(x_{1},x_{2},\lambda) = optimal - \lambda(constraint)
\end{equation}
\begin{equation}
\Delta = \begin{vmatrix}
0 & {\frac{\mathrm \partial h}{\mathrm \partial x_{1}}}& {\frac{\mathrm \partial h}{\mathrm \partial x_{2}}} \\
{\frac{\mathrm \partial h}{\mathrm \partial x_{1}}} & {\frac{\mathrm \partial^2 L}{\mathrm \partial x_{1}^2}} & {\frac{\mathrm \partial^2 L}{\mathrm \partial x_{1} \partial x_{2}}} \\
{\frac{\mathrm \partial h}{\mathrm \partial x_{2}}} & {\frac{\mathrm \partial^2 L}{\mathrm \partial x_{1} \partial x_{2}}} & {\frac{\mathrm \partial^2 L}{\mathrm \partial x_{2}^2}}
\end{vmatrix}
\end{equation}
- \Delta -> positive then maxima
- \Delta -> negative then minima
* Kuhn-Tucker with inequality constraint
** Kuhn-Tucker two variables and one inequality.
*** Kuhn-Tucker conditions
\begin{equation}
\frac{\mathrm \partial L}{\mathrm \partial x_{1}} = 0
\end{equation}
\begin{equation}
\frac{\mathrm \partial L}{\mathrm \partial x_{2}} = 0
\end{equation}
\begin{equation}
\lambda(h)=0
\end{equation}
\begin{equation}
h\leq0
\end{equation}
\begin{equation}
x_1,x_2\geq0
\end{equation}
\begin{equation}
\lambda\geq0
\end{equation}
*** Eqn
\begin{equation}
\nonumber
L(x_1,x_2,\lambda)=optimal-\lambda(constraint)
\end{equation}
\begin{equation}
\nonumber
h=constraint
\end{equation}
\begin{equation}
\nonumber
\frac{\mathrm \partial L}{\mathrm \partial x_1} = 0 => someeqn(1)
\end{equation}
\begin{equation}
\nonumber
\frac{\mathrm \partial L}{\mathrm \partial x_2} = 0 => someeqn(2)
\end{equation}
\begin{equation}
\nonumber
\lambda(h)=0=>\lambda(constraint) ..someeqn(3)
\end{equation}
\begin{equation}
\nonumber
h\leq0=>constraint\leq0 ..someeqn(4)
\end{equation}
**** Case i) \lambda=0
- put in someeqn(1) & someeqn(2)
- x_1 = & x_2 = 
- put x_1 and x_2 in Z
- if $x\neq0 then the equation is satisfy.
- if not then go for case ii)
**** Case ii) \lambda\neq0
- from someeqn(3) then
  \begin{equation}
  h = 0 .. someeqn(4)
  \end{equation}
- solve someeqn(1),(2),(4)
- x_1 = x_2= \lambda=
** Kuhn-Tucker two variables and two inequality.
*** Kuhn-Tucker conditions
\begin{equation}
\frac{\mathrm \partial L}{\mathrm \partial x_{1}} = 0
\end{equation}
\begin{equation}
\frac{\mathrm \partial L}{\mathrm \partial x_{2}} = 0
\end{equation}
\begin{equation}
\lambda_1(h_1)=0
\end{equation}
\begin{equation}
\lambda_2(h_2)=0
\end{equation}
\begin{equation}
h_1\leq0
\end{equation}
\begin{equation}
h_2\leq0
\end{equation}
\begin{equation}
x_1,x_2\geq0
\end{equation}
\begin{equation}
\lambda_1,\lambda_2\geq0
\end{equation}
*** Eqn
\begin{equation}
\nonumber
L(x_1,x_2,\lambda_1,\lambda_2)=optimal-\lambda_1(h_1)-\lambda_2(h_2)
\end{equation}
\begin{equation}
\nonumber
h_1,h_2=constraint
\end{equation}
\begin{equation}
\nonumber
\frac{\mathrm \partial L}{\mathrm \partial x_1} = 0 => someeqn(1)
\end{equation}
\begin{equation}
\nonumber
\frac{\mathrm \partial L}{\mathrm \partial x_2} = 0 => someeqn(2)
\end{equation}
\begin{equation}
\nonumber
\lambda_1(h_1)=0=>\lambda(constraint) ..someeqn(3)
\end{equation}
\begin{equation}
\nonumber
\lambda_2(h_2)=0=>\lambda(constraint) ..someeqn(4)
\end{equation}
\begin{equation}
\nonumber
h_1\leq0=>constraint\leq0 ..someeqn(5)
\end{equation}
\begin{equation}
\nonumber
h_2\leq0=>constraint\leq0 ..someeqn(6)
\end{equation}
**** Case 1> \lambda_1=0, \lambda_2=0
- Put it in (1) and (2)
- $x_1 = ? and x_2 = ?$
- Put it in (5) and (6)
**** Case 2> \lambda_1=0, \lambda_2\neq0
- Put it in (1) and (2)
- From (4) someqqn and then solve
- Put it in eqn (5) and (6)
**** Case 3> \lambda_1\neq0, \lambda_2=0
- Put it in (1) and (2)
- From (3) someqqn and then solve
- Put it in eqn (5) and (6)
**** Case 4> \lambda_1\neq0, \lambda_2\neq0
- From (3) and (4) some eqn
- put it in (1) and (2)
* TODO NLPP with two equality constraints
